src/log_lemmas.lean
@@ -1,0 +1,27 @@
+import data.nat.log
+import tactic
+
+
+namespace nat
+
+lemma log_pow_k_le (b x k : ℕ) : log b (x^k) ≤ k * (log b x + 1) :=
+begin
+  cases b, { simp, }, cases b, { simp, },
+  set b' := b.succ.succ, have one_lt : 1 < b' := by simp [b'],
+  suffices : x^k ≤ b'^(k*(log b' x+1)),
+  { refine (log_le_log_of_le this).trans _, rw log_pow one_lt, },
+  rw pow_mul', mono,
+  cases x, { exact zero_le _, },
+  apply le_of_lt, apply lt_pow_succ_log_self; simp,
+end
+
+lemma log_succ_le (b x : ℕ) : log b (x + 1) ≤ x :=
+begin
+  cases b, { simp, }, cases b, { simp, },
+  conv_rhs { rw ← @log_pow b.succ.succ (show 1 < b.succ.succ, by simp) x, },
+  apply log_monotone,
+  apply le_of_lt_succ, simp only [nat.succ_eq_add_one, add_lt_add_iff_right],
+  apply lt_pow_self, simp,
+end
+
+end nat
